iris_meta.v
@@ -1,0 +1,246 @@
+Require Import ssreflect.
+Require Import core_lang masks iris_wp.
+Require Import ModuRes.PCM ModuRes.UPred ModuRes.BI ModuRes.PreoMet ModuRes.Finmap.
+
+Module IrisMeta (RL : PCM_T) (C : CORE_LANG).
+  Module Export WP := IrisWP RL C.
+
+  Delimit Scope iris_scope with iris.
+  Local Open Scope iris_scope.
+
+  Section Adequacy.
+    Local Open Scope mask_scope.
+    Local Open Scope pcm_scope.
+    Local Open Scope bi_scope.
+    Local Open Scope lang_scope.
+    Local Open Scope list_scope.
+
+    (* weakest-pre for a threadpool *)
+    Inductive wptp (safe : bool) (m : mask) (w : Wld) (n : nat) : tpool -> list res -> list vPred -> Prop :=
+    | wp_emp : wptp safe m w n nil nil nil
+    | wp_cons e φ r tp rs φs
+              (WPE  : wp safe m e φ w n r)
+              (WPTP : wptp safe m w n tp rs φs) :
+        wptp safe m w n (e :: tp) (r :: rs) (φ :: φs).
+
+    (* Trivial lemmas about split over append *)
+    Lemma wptp_app safe m w n tp1 tp2 rs1 rs2 φs1 φs2
+          (HW1 : wptp safe m w n tp1 rs1 φs1)
+          (HW2 : wptp safe m w n tp2 rs2 φs2) :
+      wptp safe m w n (tp1 ++ tp2) (rs1 ++ rs2) (φs1 ++ φs2).
+    Proof.
+      induction HW1; [| constructor]; now trivial.
+    Qed.
+
+    Lemma wptp_app_tp safe m w n t1 t2 rs φs
+          (HW : wptp safe m w n (t1 ++ t2) rs φs) :
+      exists rs1 rs2 φs1 φs2, rs1 ++ rs2 = rs /\ φs1 ++ φs2 = φs /\ wptp safe m w n t1 rs1 φs1 /\ wptp safe m w n t2 rs2 φs2.
+    Proof.
+      revert rs φs HW; induction t1; intros; inversion HW; simpl in *; subst; clear HW.
+      - do 4 eexists. split; [|split; [|split; now econstructor] ]; reflexivity.
+      - do 4 eexists. split; [|split; [|split; now eauto using wptp] ]; reflexivity.
+      - apply IHt1 in WPTP; destruct WPTP as [rs1 [rs2 [φs1 [φs2 [EQrs [EQφs [WP1 WP2] ] ] ] ] ] ]; clear IHt1.
+        exists (r :: rs1) rs2 (φ :: φs1) φs2; simpl; subst; now auto using wptp.
+    Qed.
+
+    (* Closure under future worlds and smaller steps *)
+    Lemma wptp_closure safe m (w1 w2 : Wld) n1 n2 tp rs φs
+          (HSW : w1 ⊑ w2) (HLe : n2 <= n1)
+          (HW : wptp safe m w1 n1 tp rs φs) :
+      wptp safe m w2 n2 tp rs φs.
+    Proof.
+      induction HW; constructor; [| assumption].
+      eapply uni_pred; [eassumption | reflexivity |].
+      rewrite <- HSW; assumption.
+    Qed.
+
+    Lemma preserve_wptp safe m n k tp tp' σ σ' w rs φs
+          (HSN  : stepn n (tp, σ) (tp', σ'))
+          (HWTP : wptp safe m w (n + S k) tp rs φs)
+          (HE   : wsat σ m (comp_list rs) w @ n + S k) :
+      exists w' rs' φs',
+        w ⊑ w' /\ wptp safe m w' (S k) tp' rs' (φs ++ φs') /\ wsat σ' m (comp_list rs') w' @ S k.
+    Proof.
+      revert tp σ w rs  φs HSN HWTP HE. induction n; intros; inversion HSN; subst; clear HSN.
+      (* no step is taken *)
+      { exists w rs (@nil vPred). split; [reflexivity|]. split.
+        - rewrite List.app_nil_r. assumption.
+        - assumption.
+      }
+      inversion HS; subst; clear HS.
+      (* atomic step *)
+      { inversion H0; subst; clear H0.
+        apply wptp_app_tp in HWTP; destruct HWTP as [rs1 [rs2 [φs1 [φs2 [EQrs [EQφs [HWTP1 HWTP2] ] ] ] ] ] ].
+        inversion HWTP2; subst; clear HWTP2; rewrite ->unfold_wp in WPE.
+        edestruct (WPE w (n + S k) (comp_list (rs1 ++ rs0))) as [_ [HS _] ];
+          [reflexivity | now apply le_n | now apply mask_emp_disjoint | |].
+        + eapply wsat_equiv, HE; try reflexivity; [apply mask_emp_union |].
+          rewrite !comp_list_app; simpl comp_list; unfold equiv.
+          rewrite ->assoc, (comm (Some r)), <- assoc. reflexivity.       
+        + edestruct HS as [w' [r' [HSW [WPE' HE'] ] ] ];
+          [reflexivity | eassumption | clear WPE HS].
+          setoid_rewrite HSW. eapply IHn; clear IHn.
+          * eassumption.
+          * apply wptp_app; [eapply wptp_closure, HWTP1; [assumption | now auto with arith] |].
+            constructor; [eassumption | eapply wptp_closure, WPTP; [assumption | now auto with arith] ].
+          * eapply wsat_equiv, HE'; [now erewrite mask_emp_union| |reflexivity].
+            rewrite !comp_list_app; simpl comp_list; unfold equiv.
+            rewrite ->2!assoc, (comm (Some r')). reflexivity.
+      }
+      (* fork *)
+      inversion H; subst; clear H.
+      apply wptp_app_tp in HWTP; destruct HWTP as [rs1 [rs2 [φs1 [φs2 [EQrs [EQφs [HWTP1 HWTP2] ] ] ] ] ] ].
+      inversion HWTP2; subst; clear HWTP2; rewrite ->unfold_wp in WPE.
+      edestruct (WPE w (n + S k) (comp_list (rs1 ++ rs0))) as [_ [_ [HF _] ] ];
+        [reflexivity | now apply le_n | now apply mask_emp_disjoint | |].
+      + eapply wsat_equiv, HE; try reflexivity; [apply mask_emp_union |].
+        rewrite !comp_list_app; simpl comp_list; unfold equiv.
+        rewrite ->assoc, (comm (Some r)), <- assoc. reflexivity.
+      + specialize (HF _ _ eq_refl); destruct HF as [w' [rfk [rret [HSW [WPE' [WPS HE'] ] ] ] ] ]; clear WPE.
+        setoid_rewrite HSW. edestruct IHn as [w'' [rs'' [φs'' [HSW'' [HSWTP'' HSE''] ] ] ] ]; first eassumption; first 2 last.
+        * exists w'' rs'' ([umconst ⊤] ++ φs''). split; [eassumption|].
+          rewrite List.app_assoc. split; eassumption.
+        * rewrite -List.app_assoc. apply wptp_app; [eapply wptp_closure, HWTP1; [assumption | now auto with arith] |].
+          constructor; [eassumption|].
+          apply wptp_app; [eapply wptp_closure, WPTP; [assumption | now auto with arith] |].
+          constructor; [|now constructor]. eassumption.
+        * eapply wsat_equiv, HE'; try reflexivity; [symmetry; apply mask_emp_union |].
+          rewrite comp_list_app. simpl comp_list. rewrite !comp_list_app. simpl comp_list.
+          rewrite (comm (Some rfk) 1). erewrite pcm_op_unit by apply _. unfold equiv.
+          rewrite (comm _ (Some rfk)). rewrite ->!assoc. apply pcm_op_equiv;[|reflexivity]. unfold equiv.
+          rewrite <-assoc, (comm (Some rret)), comm. reflexivity.
+    Qed.
+
+    Lemma adequacy_ht {safe m e P Q n k tp' σ σ' w r}
+            (HT  : valid (ht safe m P e Q))
+            (HSN : stepn n ([e], σ) (tp', σ'))
+            (HP  : P w (n + S k) r)
+            (HE  : wsat σ m (Some r) w @ n + S k) :
+      exists w' rs' φs',
+        w ⊑ w' /\ wptp safe m w' (S k) tp' rs' (Q :: φs') /\ wsat σ' m (comp_list rs') w' @ S k.
+    Proof.
+      edestruct preserve_wptp with (rs:=[r]) as [w' [rs' [φs' [HSW' [HSWTP' HSWS'] ] ] ] ]; [eassumption | | simpl comp_list; erewrite comm, pcm_op_unit by apply _; eassumption | clear HT HSN HP HE].
+      - specialize (HT w (n + S k) r). apply HT in HP; try reflexivity; [|now apply unit_min].
+        econstructor; [|now econstructor]. eassumption.
+      - exists w' rs' φs'. now auto.
+    Qed.
+
+    (** This is a (relatively) generic adequacy statement for triples about an entire program: They always execute to a "good" threadpool. It does not expect the program to execute to termination.  *)
+    Theorem adequacy_glob safe m e Q tp' σ σ' k'
+            (HT  : valid (ht safe m (ownS σ) e Q))
+            (HSN : steps ([e], σ) (tp', σ')):
+      exists w' rs' φs',
+        wptp safe m w' (S k') tp' rs' (Q :: φs') /\ wsat σ' m (comp_list rs') w' @ S k'.
+    Proof.
+      destruct (steps_stepn _ _ HSN) as [n HSN']. clear HSN.
+      edestruct (adequacy_ht (w:=fdEmpty) (k:=k') (r:=(ex_own _ σ, pcm_unit _)) HT HSN') as [w' [rs' [φs' [HW [HSWTP HWS] ] ] ] ]; clear HT HSN'.
+      - exists (pcm_unit _); now rewrite ->pcm_op_unit by apply _.
+      - hnf. rewrite Plus.plus_comm. exists (fdEmpty (V:=res)). split.
+        + assert (HS : Some (ex_own _ σ, pcm_unit _) · 1 = Some (ex_own _ σ, pcm_unit _));
+          [| now setoid_rewrite HS].
+          eapply ores_equiv_eq; now erewrite comm, pcm_op_unit by apply _.
+        + intros i _; split; [reflexivity |].
+          intros _ _ [].
+      - do 3 eexists. split; [eassumption|]. assumption.
+    Qed.
+
+    Program Definition lift_vPred (Q : value -=> Prop): vPred :=
+      n[(fun v => pcmconst (mkUPred (fun n r => Q v) _))].
+    Next Obligation.
+      firstorder.
+    Qed.
+    Next Obligation.
+      intros x y H_xy P m r. simpl in H_xy. destruct n.
+      - intros LEZ. exfalso. omega.
+      - intros _. simpl. assert(H_xy': equiv x y) by assumption. rewrite H_xy'. tauto.
+    Qed.
+
+      
+    (* Adequacy as stated in the paper: for observations of the return value, after termination *)
+    Theorem adequacy_obs safe m e (Q : value -=> Prop) e' tp' σ σ'
+            (HT  : valid (ht safe m (ownS σ) e (lift_vPred Q)))
+            (HSN : steps ([e], σ) (e' :: tp', σ'))
+            (HV : is_value e') :
+        Q (exist _ e' HV).
+    Proof.
+      edestruct adequacy_glob as [w' [rs' [φs' [HSWTP HWS] ] ] ]; try eassumption.
+      inversion HSWTP; subst; clear HSWTP WPTP.
+      rewrite ->unfold_wp in WPE.
+      edestruct (WPE w' O) as [HVal _];
+        [reflexivity | unfold lt; reflexivity | now apply mask_emp_disjoint | rewrite mask_emp_union; eassumption |].
+      fold comp_list in HVal.
+      specialize (HVal HV); destruct HVal as [w'' [r'' [HSW'' [Hφ'' HE''] ] ] ].
+      destruct (Some r'' · comp_list rs) as [r''' |] eqn: EQr.
+      + assumption.
+      + exfalso. eapply wsat_not_empty, HE''. reflexivity.
+    Qed.
+
+    (* Adequacy for safe triples *)
+    Theorem adequacy_safe m e (Q : vPred) tp' σ σ' e'
+            (HT  : valid (ht true m (ownS σ) e Q))
+            (HSN : steps ([e], σ) (tp', σ'))
+            (HE  : e' ∈ tp'):
+      safeExpr e' σ'.
+    Proof.
+      edestruct adequacy_glob as [w' [rs' [φs' [HSWTP HWS] ] ] ]; try eassumption.
+      destruct (List.in_split _ _ HE) as [tp1 [tp2 HTP] ]. clear HE. subst tp'.
+      apply wptp_app_tp in HSWTP; destruct HSWTP as [rs1 [rs2 [_ [φs2 [EQrs [_ [_ HWTP2] ] ] ] ] ] ].
+      inversion HWTP2; subst; clear HWTP2 WPTP.
+      rewrite ->unfold_wp in WPE.
+      edestruct (WPE w' O) as [_ [_ [_ HSafe] ] ];
+        [reflexivity | unfold lt; reflexivity | now apply mask_emp_disjoint | |].
+      - rewrite mask_emp_union.
+        eapply wsat_equiv, HWS; try reflexivity.
+        rewrite comp_list_app. simpl comp_list.
+        rewrite ->(assoc (comp_list rs1)), ->(comm (comp_list rs1) (Some r)), <-assoc. reflexivity.
+      - apply HSafe. reflexivity.
+    Qed.
+
+  End Adequacy.
+
+  Section Lifting.
+
+    Local Open Scope mask_scope.
+    Local Open Scope pcm_scope.
+    Local Open Scope bi_scope.
+    Local Open Scope lang_scope.
+
+    Implicit Types (P : Props) (i : nat) (safe : bool) (m : mask) (e : expr) (Q R : vPred) (r : res).
+
+
+    Program Definition lift_ePred (φ : expr -=> Prop) : expr -n> Props :=
+      n[(fun v => pcmconst (mkUPred (fun n r => φ v) _))].
+    Next Obligation.
+      firstorder.
+    Qed.
+    Next Obligation.
+      intros x y H_xy P m r. simpl in H_xy. destruct n.
+      - intros LEZ. exfalso. omega.
+      - intros _. simpl. assert(H_xy': equiv x y) by assumption. rewrite H_xy'. tauto.
+    Qed.
+
+    Program Definition plugExpr safe m φ P Q: expr -n> Props :=
+      n[(fun e => (lift_ePred φ e) ∨ (ht safe m P e Q))].
+    Next Obligation.
+      intros e1 e2 Heq w n' r HLt.
+      destruct n as [|n]; [now inversion HLt | simpl in *].
+      subst e2; tauto.
+    Qed.
+
+    Theorem lift_pure_step safe m e (φ : expr -=> Prop) P Q
+            (RED  : reducible e)
+            (STEP : forall σ e2 σ2, prim_step (e, σ) (e2, σ2) -> σ2 = σ /\ φ e2):
+      (all (plugExpr safe m φ P Q)) ⊑ ht safe m (▹P) e Q.
+    Proof.
+    Admitted.
+
+    Lemma lift_pure_deterministic_step safe m e e' P Q
+          (RED  : reducible e)
+          (STEP : forall σ e2 σ2, prim_step (e, σ) (e2, σ2) -> σ2 = σ /\ e2 = e):
+      ht safe m P e' Q ⊑ ht safe m (▹P) e Q.
+    Proof.
+    Admitted.
+
+  End Lifting. 
+
+End IrisMeta.
